NCML.lean
@@ -2,7 +2,6 @@ module  -- shake: keep-all --deprecated_module: ignore
 
 public import NCML.CK.Axioms.BBox
 public import NCML.CK.Axioms.BDia
-public import NCML.CK.Axioms.TBox
 public import NCML.CK.Axioms.TDia
 public import NCML.CK.CKB_IKB
 public import NCML.CK.Canonical
@@ -13,9 +12,12 @@ public import NCML.CK.Countermodel.TDia
 public import NCML.CK.Frame.BackwardConfluent
 public import NCML.CK.Frame.ForwardConfluent
 public import NCML.CK.Frame.FrameClass
+public import NCML.CK.Frame.ReflexiveMComp
+public import NCML.CK.Frame.ReturningMRel
 public import NCML.CK.Frame.SerialMRel
 public import NCML.CK.Frame.SymmetricMRel
 public import NCML.CK.Logic.CKD
+public import NCML.CK.Logic.CKTBox
 public import NCML.CK.Semantics
 public import NCML.CK.Soundness
 public import NCML.Formula
