NCML/CK/Frame/ReturningMRel.lean
@@ -1,0 +1,30 @@
+module
+
+public import NCML.CK.Frame.ReflexiveMComp
+
+@[expose] public section
+
+namespace CK
+
+variable {κ : Type*}
+
+namespace Frame
+
+variable {F : Frame κ}
+
+class ReturningMRel (F : Frame κ) : Prop where
+  returning_mRel : ∀ x : F.World, ∃ y, x ≼ y ∧ y ⊏ x
+
+export ReturningMRel (returning_mRel)
+
+instance [F.ReturningMRel] : F.ReflexiveMComp where
+  reflexive_mComp x := by
+    obtain ⟨y, Ixy, Myx⟩ := returning_mRel x;
+    right;
+    exact ⟨y, x, Ixy, Myx, refl x⟩;
+
+end Frame
+
+end CK
+
+end
